src/mebi_utils.ml
@@ -119,13 +119,13 @@ let encode_econstr (t : EConstr.t) : E.t mm = encode t
 let encode_constrexpr (t : Constrexpr.constr_expr) : E.t mm =
   Log.debug "mebi_utils.encode_constrexpr";
   let open Mebi_wrapper.Syntax in
-  let* (t' : EConstr.t) = constrexpr_to_econstr t in
+  let* t' : EConstr.t = constrexpr_to_econstr t in
   encode_econstr t'
 ;;
 
 let encode_ref (t : Libnames.qualid) : E.t mm =
   Log.debug "mebi_utils.encode_ref";
   let open Mebi_wrapper.Syntax in
-  let* (info : Mebi_ind.info) = get_ind_info (ref_to_glob t) in
+  let* info : Mebi_ind.info = get_ind_info (ref_to_glob t) in
   encode_econstr info.name
 ;;
