examples/bisimilarity/CADP/Glued.v
@@ -1,0 +1,212 @@
+Require Import MEBI.Examples.CADP.
+
+Import Protocol.
+
+Definition do_acquire_inner (c:tm) (s:state) (r:resource)
+  : composition
+  :=
+  let e : env := (s, r) in
+  (* REC_DEF 2 *)
+  let t : tm := unfold (AcquireInnerDef, AcquireInnerBody) AcquireInnerBody in
+  (* ACT READ_LOCKED *)
+  match read_locked e with
+  | None => (PRC ERR
+                (add_error (Build_error 40
+                  "do_acquire_inner, read_locked e failed" (Build_error_info None (None, None))) s),
+                r)
+  | Some e =>
+    (* IF (VAR LOCKED) *)
+    match (get_local_var_value LOCKED (get_state e)) with
+    | BOOL true => (* REC_CALL 2 *) (PRC (SEQ t c) (get_state e), get_resource e)
+    | BOOL false => (PRC c (get_state e), get_resource e)
+    | _ => (PRC ERR
+                (add_error (Build_error 41
+                  "do_acquire_inner, var locked not bool" (Build_error_info None (None, None))) (get_state e)),
+                get_resource e)
+    end
+  end
+  .
+
+
+Definition do_acquire (c:tm) (s:state) (r:resource)
+  : composition
+  :=
+  let e : env := (s, r) in
+  (* ACT (WRITE_NEXT THE_PID NIL) *)
+  match write_next THE_PID NIL e with
+  | None => (PRC ERR
+                (add_error (Build_error 50
+                  "do_acquire, write_next THE_PID NIL failed" (Build_error_info None (None, None))) s),
+                r)
+  | Some e =>
+    (* ACT FETCH_AND_STORE *)
+    match fetch_and_store e with
+    | None => (PRC ERR
+                  (add_error (Build_error 51
+                    "do_acquire, fetch_and_store failed" (Build_error_info None (None, None))) (get_state e)),
+                  (get_resource e))
+    | Some e =>
+      (* IF (EQ (VAR PREDECESSOR) (VAL NIL)) *)
+      match (get_local_var_value PREDECESSOR (get_state e)) with
+      | NIL => (* OK *) (PRC c (get_state e), get_resource e)
+      | _ =>
+        (* ACT (WRITE_LOCKED THE_PID (BOOL true)) *)
+        match write_locked THE_PID (BOOL true) e with
+        | None => (PRC ERR
+                      (add_error (Build_error 52
+                        "do_acquire, write_locked THE_PID (BOOL true) failed" (Build_error_info None (None, None))) (get_state e)),
+                  (get_resource e))
+        | Some e =>
+          (* ACT (WRITE_NEXT PREDECESSOR (GET THE_PID)) *)
+          match write_next PREDECESSOR (GET THE_PID) e with
+          | None => (PRC ERR
+                        (add_error (Build_error 53
+                          "do_acquire, write_next PREDECESSOR (GET THE_PID) failed" (Build_error_info None (None, None))) (get_state e)),
+                    (get_resource e))
+          | Some e =>
+            (PRC (SEQ (AcquireInnerLoop) c) (get_state e)
+            , get_resource e
+            )
+          end
+        end
+      end
+    end
+  end
+  .
+
+Definition do_release_inner (c:tm) (s:state) (r:resource)
+  : composition
+  :=
+  let e : env := (s, r) in
+  (* REC_DEF 1 *)
+  let t : tm := unfold (ReleaseInnerDef, ReleaseInnerBody) ReleaseInnerBody in
+  (* ACT READ_NEXT *)
+  match read_next e with
+  | None => (PRC ERR
+                (add_error (Build_error 45
+                  "do_release_inner, read_next e failed" (Build_error_info None (None, None))) s),
+                r)
+  | Some e =>
+    (* IF (EQ (VAL NIL) (VAR NEXT)) *)
+    match (get_local_var_value NEXT (get_state e)) with
+    | NIL => (* REC_CALL 1 *) (PRC (SEQ t c) (get_state e), get_resource e)
+    | _ =>
+      (* ACT (WRITE_LOCKED NEXT (BOOL false)) *)
+      match write_locked NEXT (BOOL false) e with
+      | None => (PRC ERR
+                    (add_error (Build_error 46
+                      "do_release_inner, write_locked NEXT (BOOL false) failed" (Build_error_info None (None, None))) (get_state e)),
+                    (get_resource e))
+      | Some e =>
+        (PRC c (get_state e), get_resource e)
+      end
+    end
+  end
+  .
+
+Definition do_release (c:tm) (s:state) (r:resource)
+  : composition
+  :=
+  let e : env := (s, r) in
+  (* ACT READ_NEXT *)
+  match read_next e with
+  | None => (PRC ERR
+                (add_error (Build_error 60
+                  "do_release, read_next e failed" (Build_error_info None (None, None))) s),
+                r)
+  | Some e =>
+    (* IF (EQ (VAL NIL) (VAR NEXT)) *)
+    match (get_local_var_value NEXT (get_state e)) with
+    | NIL =>
+      (* ACT COMPARE_AND_SWAP *)
+      match compare_and_swap e with
+      | None => (PRC ERR
+                    (add_error (Build_error 61
+                      "do_acquire, compare_and_swap failed" (Build_error_info None (None, None))) (get_state e)),
+                    (get_resource e))
+      | Some e =>
+        (* IF (EQ FLS (VAR SWAP)) *)
+        match (get_local_var_value SWAP (get_state e)) with
+        | BOOL false =>
+          (PRC (SEQ (ReleaseInnerLoop) c) (get_state e)
+          , get_resource e)
+        | _ => (* OK *) (PRC c (get_state e), get_resource e)
+        end
+      end
+
+    | _ =>
+      (* ACT (WRITE_LOCKED NEXT (BOOL false)) *)
+      match write_locked NEXT (BOOL false) e with
+      | None => (PRC ERR
+                    (add_error (Build_error 61
+                      "do_release, write_locked NEXT (BOOL false) failed" (Build_error_info None (None, None))) (get_state e)),
+                    (get_resource e))
+      | Some e =>
+        (PRC c (get_state e), get_resource e)
+      end
+    end
+  end
+  .
+
+
+Definition do_main_loop (b:tm) (s:state) (r:resource)
+  : composition
+  :=
+  (* REC_DEF 0 *)
+  (PRC (unfold (PMainLoopDef, b) b) s, r)
+  .
+
+Inductive bigstep : composition -> option label -> composition -> Prop :=
+(*  0 *)
+| DO_MAIN_LOOP : forall b s r,
+  bigstep (PRC (REC_DEF PMainLoopDef b) s, r) 
+          None 
+          (do_main_loop b s r)
+
+(*  1 *)
+| DO_ACQUIRE : forall c s r,
+  bigstep (PRC (SEQ (Acquire) (c)) s, r)
+          None
+          (do_acquire c s r)
+
+(*  2 *)
+| DO_RELEASE : forall c s r,
+  bigstep (PRC (SEQ (Release) (c)) s, r)
+          None
+          (do_release c s r)
+
+(*  3 *)
+| DO_ACQUIRE_INNER : forall c s r,
+  bigstep (PRC (SEQ (AcquireInnerLoop) c) s, r)
+          None
+          (do_acquire_inner c s r)
+
+(*  4 *)
+| DO_RELEASE_INNER : forall c s r,
+  bigstep (PRC (SEQ (ReleaseInnerLoop) c) s, r)
+          None
+          (do_release_inner c s r)
+
+(*  5 *)
+| DO_SEQ_ACT_ENTER : forall y s r,
+  bigstep (PRC (SEQ (ACT ENTER) y) s, r) 
+          (Some (ENTER, (get_pid s))) 
+          (PRC y s, r)
+
+(*  6 *)
+| DO_SEQ_ACT_LEAVE : forall y s r,
+  bigstep (PRC (SEQ (ACT LEAVE) y) s, r) 
+          (Some (LEAVE, (get_pid s))) 
+          (PRC y s, r)
+
+(*  7 *)
+| DO_PAR_L : forall a l1 l2 r gr1 gr2,
+  bigstep (l1, gr1) a (l2, gr2) ->
+  bigstep (PAR l1 r, gr1) a (PAR l2 r, gr2)
+
+(*  8 *)
+| DO_PAR_R : forall a l r1 r2 gr1 gr2,
+  bigstep (r1, gr1) a (r2, gr2) ->
+  bigstep (PAR l r1, gr1) a (PAR l r2, gr2)
+
+.
