examples/bisimilarity/CADP/Size1/PluginTest.v
@@ -1,0 +1,37 @@
+Require Import MEBI.loader.
+Require Coq.Program.Tactics.
+
+Require Import Relation_Definitions.
+Require Import Relation_Operators.
+Require Operators_Properties.
+
+Require Import MEBI.Bisimilarity.
+Require Import MEBI.Examples.CADP.
+Import Protocol.
+
+Require Import MEBI.Examples.bisimilarity.CADP.Glued.
+
+MeBi Divider "Examples.Bisimilarity.CADP.Size1.PluginTest".
+MeBi Reset All.
+MeBi Set Bound 100.
+MeBi Set Weak Option label.
+
+(* MeBi Set ShowDebug True. *)
+(* MeBi Set ShowDetails True. *)
+
+MeBi Divider "Examples.Bisimilarity.CADP.Size1.PluginTest.Term".
+Example p1 : tm * env := (P, Env.initial 1).
+MeBi FSM p1 Using step.
+MeBi Minimize p1 Using step.
+
+MeBi Divider "Examples.Bisimilarity.CADP.Size1.PluginTest.Composition".
+Example c1 : composition := compose (create 1 P).
+MeBi FSM c1 Using lts step.
+MeBi Minimize c1 Using lts step.
+
+MeBi Divider "Examples.Bisimilarity.CADP.Size1.PluginTest.Glued".
+MeBi FSM c1 Using bigstep lts step.
+MeBi Minimize c1 Using bigstep lts step.
+
+MeBi Divider "Examples.Bisimilarity.CADP.Size1.PluginTest.Bisim".
+MeBi Bisim c1 With bigstep And c1 With lts Using step.
